disk-betree/ImplModelCache.i.dfy
@@ -20,7 +20,7 @@ module ImplModelCache {
   predicate RefAvailable(s: Variables, ref: Reference)
   {
     && s.Ready?
-    && ref !in s.ephemeralIndirectionTable.contents
+    && ref !in s.ephemeralIndirectionTable.graph
     && ref !in s.cache 
     && ref != BT.G.Root()
   }
@@ -32,7 +32,7 @@ module ImplModelCache {
   ensures ref.Some? ==> RefAvailable(s, ref.value)
   decreases 0x1_0000_0000_0000_0000 - i as int
   {
-    if i !in s.ephemeralIndirectionTable.contents && i !in s.cache then (
+    if i !in s.ephemeralIndirectionTable.graph && i !in s.cache then (
       Some(i)
     ) else if i == 0xffff_ffff_ffff_ffff then (
       None
@@ -57,7 +57,7 @@ module ImplModelCache {
   ensures ref.Some? ==> ref.value != avoid
   decreases 0x1_0000_0000_0000_0000 - i as int
   {
-    if i != avoid && i !in s.ephemeralIndirectionTable.contents && i !in s.cache then (
+    if i != avoid && i !in s.ephemeralIndirectionTable.graph && i !in s.cache then (
       Some(i)
     ) else if i == 0xffff_ffff_ffff_ffff then (
       None
@@ -79,7 +79,7 @@ module ImplModelCache {
   predicate WriteAllocConditions(k: Constants, s: Variables)
   {
     && s.Ready?
-    && MutableMapModel.Inv(s.ephemeralIndirectionTable)
+    && IndirectionTableModel.Inv(s.ephemeralIndirectionTable)
     && (forall loc |
         loc in IIndirectionTable(s.ephemeralIndirectionTable).locs.Values :: 
           BC.ValidLocationForNode(loc))
@@ -92,15 +92,15 @@ module ImplModelCache {
 
   lemma lemmaIndirectionTableLocIndexValid(k: Constants, s: Variables, ref: BT.G.Reference)
   requires WriteAllocConditions(k, s)
-  ensures ref in s.ephemeralIndirectionTable.contents && s.ephemeralIndirectionTable.contents[ref].0.Some? ==>
+  ensures ref in s.ephemeralIndirectionTable.locs ==>
     (
-      && 0 <= s.ephemeralIndirectionTable.contents[ref].0.value.addr as int / BlockSize() < NumBlocks()
-      && (s.ephemeralIndirectionTable.contents[ref].0.value.addr as int / BlockSize()) * BlockSize() == s.ephemeralIndirectionTable.contents[ref].0.value.addr as int
+      && 0 <= s.ephemeralIndirectionTable.locs[ref].addr as int / BlockSize() < NumBlocks()
+      && (s.ephemeralIndirectionTable.locs[ref].addr as int / BlockSize()) * BlockSize() == s.ephemeralIndirectionTable.locs[ref].addr as int
     )
   {
-    if ref in s.ephemeralIndirectionTable.contents && s.ephemeralIndirectionTable.contents[ref].0.Some? {
+    if ref in s.ephemeralIndirectionTable.locs {
       reveal_ConsistentBitmap();
-      var loc := s.ephemeralIndirectionTable.contents[ref].0.value;
+      var loc := s.ephemeralIndirectionTable.locs[ref];
       var i := loc.addr as int / BlockSize();
       assert IIndirectionTable(s.ephemeralIndirectionTable).locs[ref] == loc;
       assert loc in IIndirectionTable(s.ephemeralIndirectionTable).locs.Values;
@@ -122,19 +122,18 @@ module ImplModelCache {
   ensures WriteAllocConditions(k, s')
   {
     lemmaIndirectionTableLocIndexValid(k, s, ref);
-    assume s.ephemeralIndirectionTable.count as nat < 0x10000000000000000 / 8;
-    var (eph, oldEntry) := MutableMapModel.InsertAndGetOld(s.ephemeralIndirectionTable, ref,
-        (None, if children.Some? then children.value else []));
-    var blockAllocator' := if oldEntry.Some? && oldEntry.value.0.Some?
-      then ImplModelBlockAllocator.MarkFreeEphemeral(s.blockAllocator, oldEntry.value.0.value.addr as int / BlockSize())
+    var (eph, oldLoc) := IndirectionTableModel.UpdateAndRemoveLoc(s.ephemeralIndirectionTable, ref,
+        (if children.Some? then children.value else []));
+    var blockAllocator' := if oldLoc.Some?
+      then ImplModelBlockAllocator.MarkFreeEphemeral(s.blockAllocator, oldLoc.value.addr as int / BlockSize())
       else s.blockAllocator;
     var s' := s.(ephemeralIndirectionTable := eph)
      .(lru := LruModel.Use(s.lru, ref))
      .(blockAllocator := blockAllocator');
 
     freeIndirectionTableLocCorrect(k, s, s', ref,
-      if oldEntry.Some? && oldEntry.value.0.Some?
-      then Some(oldEntry.value.0.value.addr as int / BlockSize())
+      if oldLoc.Some?
+      then Some(oldLoc.value.addr as int / BlockSize())
       else None);
     reveal_ConsistentBitmap();
 
@@ -168,19 +167,18 @@ module ImplModelCache {
   ensures WriteAllocConditions(k, s')
   {
     lemmaIndirectionTableLocIndexValid(k, s, ref);
-    assume s.ephemeralIndirectionTable.count as nat < 0x10000000000000000 / 8;
-    var (eph, oldEntry) := MutableMapModel.InsertAndGetOld(s.ephemeralIndirectionTable, ref,
-        (None, if node.children.Some? then node.children.value else []));
-    var blockAllocator' := if oldEntry.Some? && oldEntry.value.0.Some?
-      then ImplModelBlockAllocator.MarkFreeEphemeral(s.blockAllocator, oldEntry.value.0.value.addr as int / BlockSize())
+    var (eph, oldLoc) := IndirectionTableModel.UpdateAndRemoveLoc(s.ephemeralIndirectionTable, ref,
+        (if node.children.Some? then node.children.value else []));
+    var blockAllocator' := if oldLoc.Some?
+      then ImplModelBlockAllocator.MarkFreeEphemeral(s.blockAllocator, oldLoc.value.addr as int / BlockSize())
       else s.blockAllocator;
     var s' := s.(ephemeralIndirectionTable := eph).(cache := s.cache[ref := node])
         .(lru := LruModel.Use(s.lru, ref))
         .(blockAllocator := blockAllocator');
 
     freeIndirectionTableLocCorrect(k, s, s', ref,
-      if oldEntry.Some? && oldEntry.value.0.Some?
-      then Some(oldEntry.value.0.value.addr as int / BlockSize())
+      if oldLoc.Some?
+      then Some(oldLoc.value.addr as int / BlockSize())
       else None);
     reveal_ConsistentBitmap();
 
@@ -257,8 +255,8 @@ module ImplModelCache {
         if i == 0 {
           assert false;
         } else {
-          var r :| r in s'.ephemeralIndirectionTable.contents && s'.ephemeralIndirectionTable.contents[r].0.Some? &&
-              s'.ephemeralIndirectionTable.contents[r].0.value.addr as int == i * BlockSize() as int;
+          var r :| r in s'.ephemeralIndirectionTable.locs &&
+              s'.ephemeralIndirectionTable.locs[r].addr as int == i * BlockSize() as int;
           assert MapsAgreeOnKey(
             IIndirectionTable(s.ephemeralIndirectionTable).locs,
             IIndirectionTable(s'.ephemeralIndirectionTable).locs, r);
@@ -279,8 +277,8 @@ module ImplModelCache {
           assert IsLocAllocBitmap(s.blockAllocator.ephemeral, i);
           assert IsLocAllocBitmap(s'.blockAllocator.ephemeral, i);
         } else {
-          var r :| r in s'.ephemeralIndirectionTable.contents && s'.ephemeralIndirectionTable.contents[r].0.Some? &&
-              s'.ephemeralIndirectionTable.contents[r].0.value.addr as int == i * BlockSize() as int;
+          var r :| r in s'.ephemeralIndirectionTable.locs &&
+              s'.ephemeralIndirectionTable.locs[r].addr as int == i * BlockSize() as int;
           //assert r != ref;
           assert MapsAgreeOnKey(
             IIndirectionTable(s.ephemeralIndirectionTable).locs,
@@ -309,13 +307,13 @@ module ImplModelCache {
         if i == 0 {
           assert IsLocAllocIndirectionTable(s'.ephemeralIndirectionTable, i);
         } else {
-          var r :| r in s.ephemeralIndirectionTable.contents && s.ephemeralIndirectionTable.contents[r].0.Some? &&
-            s.ephemeralIndirectionTable.contents[r].0.value.addr as int == i * BlockSize() as int;
+          var r :| r in s.ephemeralIndirectionTable.locs &&
+            s.ephemeralIndirectionTable.locs[r].addr as int == i * BlockSize() as int;
           assert MapsAgreeOnKey(
             IIndirectionTable(s.ephemeralIndirectionTable).locs,
             IIndirectionTable(s'.ephemeralIndirectionTable).locs, r);
-          assert r in s'.ephemeralIndirectionTable.contents && s'.ephemeralIndirectionTable.contents[r].0.Some? &&
-            s'.ephemeralIndirectionTable.contents[r].0.value.addr as int == i * BlockSize() as int;
+          assert r in s'.ephemeralIndirectionTable.locs &&
+            s'.ephemeralIndirectionTable.locs[r].addr as int == i * BlockSize() as int;
           assert IsLocAllocIndirectionTable(s'.ephemeralIndirectionTable, i);
         }
       }
@@ -383,6 +381,8 @@ module ImplModelCache {
       LruModel.LruUse(s.lru, ref.value);
       writeBookkeepingBitmapCorrect(k, s, ref.value, node.children);
       reveal_writeBookkeeping();
+
+      var (s', ref0) := allocWithNode(k, s, node);
     }
   }
   
@@ -394,7 +394,7 @@ module ImplModelCache {
   requires ref in s.cache
   requires WFNode(node)
   requires BC.BlockPointsToValidReferences(INode(node), IIndirectionTable(s.ephemeralIndirectionTable).graph)
-  requires s.frozenIndirectionTable.Some? && ref in s.frozenIndirectionTable.value.contents ==> s.frozenIndirectionTable.value.contents[ref].0.Some?
+  requires s.frozenIndirectionTable.Some? && ref in s.frozenIndirectionTable.value.graph ==> ref in s.frozenIndirectionTable.value.locs
   ensures var s' := writeWithNode(k, s, ref, node);
     && WFVars(s')
     && BC.Dirty(Ik(k), IVars(s), IVars(s'), ref, INode(node))
@@ -437,9 +437,9 @@ module ImplModelCache {
   requires s.Ready?
   requires Inv(k, s)
   requires ref in s.cache
-  requires ref in s.ephemeralIndirectionTable.contents
+  requires ref in s.ephemeralIndirectionTable.graph
   requires childref in BT.G.Successors(INode(s.cache[ref]))
-  ensures childref in s.ephemeralIndirectionTable.contents
+  ensures childref in s.ephemeralIndirectionTable.graph
   {
     assert childref in IIndirectionTable(s.ephemeralIndirectionTable).graph[ref];
   }
@@ -447,15 +447,15 @@ module ImplModelCache {
   lemma lemmaGraphChildInGraph(k: Constants, s: Variables, ref: BT.G.Reference, childref: BT.G.Reference)
   requires s.Ready?
   requires Inv(k, s)
-  requires ref in s.ephemeralIndirectionTable.contents
-  requires childref in s.ephemeralIndirectionTable.contents[ref].1
-  ensures childref in s.ephemeralIndirectionTable.contents
+  requires ref in s.ephemeralIndirectionTable.graph
+  requires childref in s.ephemeralIndirectionTable.graph[ref]
+  ensures childref in s.ephemeralIndirectionTable.graph
 
   lemma lemmaBlockPointsToValidReferences(k: Constants, s: Variables, ref: BT.G.Reference)
   requires Inv(k, s)
   requires s.Ready?
   requires ref in s.cache
-  requires ref in s.ephemeralIndirectionTable.contents
+  requires ref in s.ephemeralIndirectionTable.graph
   ensures BC.BlockPointsToValidReferences(INode(s.cache[ref]), IIndirectionTable(s.ephemeralIndirectionTable).graph);
   {
     var node := INode(s.cache[ref]);
